\subsection{Wavlengths Average Absorption}

\begin{align}
	\dfrac{d I(\lambda)}{ds} = - I(\lambda) \kappa(\lambda)
\end{align}
The absorption is a sum of line absorptions:
\begin{align}
	\kappa(\lambda) = \sum_i \kappa_i(\lambda_i) f_i(\lambda)
\end{align}
Integrating over wavelengths:
\begin{align}
	\dfrac{d}{ds} \int_{\Delta \lambda} I(\lambda) d \lambda = - \sum_i  \int_{\Delta \lambda} I(\lambda) \kappa_i(\lambda_i) f_i(\lambda)  d \lambda
\end{align}
Assuming that the intensity is constant within the integration intervall:
\begin{align}
    \dfrac{d I}{ds} &= - \dfrac{I}{\Delta \lambda} \sum_i \kappa_i(\lambda_i)  \int_{\Delta \lambda}  f_i(\lambda)  d \lambda \\
                    &= - \dfrac{I}{\Delta \lambda} \sum_i \kappa_i(\lambda_i)
\end{align}
Integrating along the path:
\begin{align}
	\dfrac{dI}{I} = - \dfrac{1}{\Delta \lambda} \sum_i \kappa_i(\lambda_i) ds
\end{align}
yields:
\begin{align}
	\ln \dfrac{I(z)}{I(z_0)} = - \dfrac{1}{\Delta \lambda} \int_{z_0}^{z} \sum_i \kappa_i(\lambda_i) ds
\end{align}
and finally:
\begin{align}
	I(z) = I(z_0) \exp\left( - \dfrac{1}{\Delta \lambda} \int_{z_0}^{z} \sum_i \kappa_i(\lambda_i) ds \right)
\end{align}
With $\int_{z_0}^{z} \sum_i \kappa_i(\lambda_i) ds \approx 2 10^{-3}$ the intensity at TOA is near zero, that means all the intensity is absorbed.
This of course is wrong. The false assumption is that the intensity along the path in the atmosphere is independent of wavelength.

\subsection{Reinhart}

Equation (8) and (9):
\begin{align}
    dI_a(u_j) = S_0 f(u_j) \Delta u_j \left(1 - \exp\left(-\int \alpha(\rho, u_j) d \rho\right) \right) 2 \pi \cos \theta \sin \theta d \theta
\end{align}
In Reinhart the expression for $\alpha(\rho, u_j)$ is not explicitely given, so the value of $\kappa_i$ as defined above is taken.
\begin{align}
    f(u) &= \dfrac{15}{\pi^4} \dfrac{u^3}{\exp(u) - 1} \\
    u    &= \dfrac{h \nu}{k_B T} \\
    S_0  &= \sigma T^4
\end{align}
If $\exp\left(-\int \alpha(\rho, u_j) d \rho\right)$ only depends slightly on the angle $\theta$ the integral over $theta$ is:
\begin{align}
    \int_{0}^{\pi/2} 2 \pi \cos \theta \sin \theta d \theta = \pi
\end{align}
Sum over all lines:
\begin{align}
    F = \sum_j I_a(u_j) = \sum_j S_0 f(u_j) \Delta u_j \left(1 - \exp\left(-\int \alpha(\rho, u_j) d \rho\right) \right)
\end{align}
The sum $F =  \pi S_0 \sum_j f(u_j) \Delta u_j$ has to equal the intensity emitted from the earth surface.
Assuming $f(u_j) \Delta u_j$ approximately constant:
\begin{align}
    \sum_j \left(1 - \exp\left(-\int \alpha(\rho, u_j) d \rho\right) \right)
\end{align}
is the relative absorption. The value in the line intervall $[12-18 \mu m]$ is $1.8 10^{-3}$ at 400 ppm $CO_2$ and $3.6  10^{-3}$ at 800 ppm $CO_2$.
If instead of $\kappa_i$ $\kappa_i / \Delta \lambda$ is taken for $\alpha$ the values are $2.4 10^4$ and $2.8 10^4$ respectively.
The integral

If the angle between surface normal and the path direction is $\theta$ the path lngth as function of the height $z$ measured from 
the surface is given by:

\begin{align}
	s = \dfrac{z}{\cos\theta}
\end{align}
Assuming constant $\kappa$ and $\epsilon$ in \eqn{eqn1} the solution is given by:
\begin{align}
	I = c(s) \exp( - \kappa s)
\end{align}
Inserting into \eqn{eqn1} yields:
\begin{align}
		\dfrac{d I}{d s} = \dfrac{d c(s)}{ds } \exp( - \kappa s) - \kappa c(s) \exp( - \kappa s) = - \kappa c(s) \exp( - \kappa s) + \epsilon
\end{align}
and:
\begin{align}
	\dfrac{d c(s)}{ds}  = \epsilon \exp(\kappa s)
\end{align}
Transforming
\begin{align}
	\dfrac{d c(s)}{\epsilon}  =  \exp(\kappa s) ds
\end{align}

\begin{align}
	\int_{c_0}^c \dfrac{d c(s)}{\epsilon}  =  \int_0^z \exp(\kappa s) ds
\end{align}

\begin{align}
	\dfrac{c - c_0}{\epsilon}  = \dfrac{1}{\kappa} \left(\exp(\kappa z) - 1\right)
\end{align}

\begin{align}
	c = c_0 + \epsilon \dfrac{1}{\kappa} \left(\exp(\kappa z) - 1\right)
\end{align}

\begin{align}
	I = c_0 \exp( - \kappa z) + \epsilon \dfrac{1}{\kappa} \left(1 - \exp( - \kappa z)\right)
\end{align}

\begin{align}
	I = I(0) \exp( - \kappa z) +  \dfrac{\epsilon}{\kappa} \left(1 - \exp( - \kappa z)\right)
\end{align}

