
\section{Integration of the Radiation Transfer Equation}
\label{app_a_1}

The radiation transfer equation \eqn{eqn1} is of the form:
\begin{align}
	\label{eqn_a_rte}
	\dfrac{dy}{dx} = - a y + b
\end{align}
If $a$ and $b$ are constant the solution can be written as:
\begin{align}
	y(x) = c(x) \exp( - a x)
\end{align}
Inserting into \eqn{eqn_a_rte} yields:
\begin{align}
		\dfrac{d y}{d x} = \dfrac{d c(x)}{dx} \exp( - a x) - a c(x) \exp( - a x) = - a c(x) \exp( - a x) + b
\end{align}
and further:
\begin{align}
	\dfrac{d c(x)}{dx}  = b \exp(a x)
\end{align}
This can be integrated:
\begin{align}
	d c(x) = b \exp(a x) dx
\end{align}
\begin{align}
	\int_{c_0}^c d c(x)  =  b \int_0^x \exp(a x) dx
\end{align}
\begin{align}
	c - c_0  = \dfrac{b}{a} \left(\exp(a x) - 1\right)
\end{align}
And finally:
\begin{align}
	y(x) = y(0) \exp( - a x) + \dfrac{b}{a} \left(1 - \exp( - a x)\right)
\end{align}

\section{Cubic Polynomial Interpolation}
\label{app_a_2}
\begin{align}
	y(x) = a_0 + a_1 x + a_2 x^2 +  a_3 x^3
\end{align}

With $a_0 = y(0)$ and $\dfrac{d y(0)}{d x} = 0$ it follows that $a_1 = 0$.
The coefficients $a_2$ and $a_3$ are determined by the linear system: 
\begin{align}
	y(x_1) &= y(0) + a_2 x_1^2 +  a_3 x_1^3 \\
	y(x_2) &= y(0) + a_2 x_2^2 +  a_3 x_2^3
\end{align}
which can be written as matrix equation:
\begin{align}x
	\begin{pmatrix} x_1^2 & x_1^3 \\
					x_2^2 & x_2^3 
	\end{pmatrix}
	\begin{pmatrix}	a_2 \\ a_3
	\end{pmatrix}
	=
	\begin{pmatrix} y(x_1) - y(0) \\ y(x_2) - y(0)
	\end{pmatrix}
\end{align}
Using Cramer's rule the solution is given by:
\begin{align}
 a_2 &= \dfrac{(y(x_1) - y(0)) x_2^3 - (y(x_2) - y(0)) x_1^3}{x_1^2 x_2^3 - x_1^3 x_2^2} \\
 a_3 &= \dfrac{(y(x_2) - y(0)) x_1^2 - (y(x_1) - y(0)) x_2^2}{x_1^2 x_2^3 - x_1^3 x_2^2}
\end{align}

\section{Line Shapes}

\subsection{Gaussian Lineshape}

\begin{align}
	\dfrac{\Delta \lambda}{\lambda} = \dfrac{v}{c} = \dfrac{1}{c} \sqrt{\dfrac{2 k_B T}{m}}
\end{align}

\begin{align}
	\exp(-a x_h^2) &= \dfrac{1}{2} \\
	-a x_h^2 &= \ln{\dfrac{1}{2}} \\
	a &= \dfrac{\ln{2}}{x_h^2}
\end{align}

\begin{align}
	x_h = x_{hwhm} = \Delta \lambda
\end{align}

\begin{align}
	a &= \dfrac{\ln{2}}{\Delta \lambda^2}
\end{align}

\begin{align}
	\int \exp\left(- \dfrac{\ln{2}}{\Delta \lambda^2} x^2\right) dx = \sqrt{\dfrac{\pi}{a}}
\end{align}

\begin{align}
	\sqrt{\dfrac{a}{\pi}} \int \exp\left(- \dfrac{\ln{2}}{\Delta \lambda^2} x^2\right) dx = 1
\end{align}

\begin{align}
	\sqrt{\dfrac{\dfrac{\ln{2}}{\Delta \lambda^2}}{\pi}} \int \exp\left(- \dfrac{\ln{2}}{\Delta \lambda^2} x^2\right) dx = 1
\end{align}

\begin{align}
	&\Delta \lambda = \dfrac{1}{c} \sqrt{\dfrac{2 k_B T}{m}} \lambda \\
	&\sqrt{\dfrac{\ln{2}}{\pi \Delta \lambda^2}} \int \exp\left(- \dfrac{\ln{2}}{\Delta \lambda^2} (\lambda - \lambda_0)^2\right) dx = 1
\end{align}

\subsection{Lorentz Lineshape}

\begin{align}
	L(\nu) = \dfrac{a^2}{ (\nu - \nu_0)^2 + a^2}
\end{align}

\begin{align}
	L(\nu_0) = 1
\end{align}

\begin{align}
	L(\nu_h) = 1/2  = \dfrac{a^2}{ (\nu_h - \nu_0)^2 + a^2}
\end{align}

\begin{align}
	 (\nu_h - \nu_0)^2 + a^2 = 2 a^2
\end{align}

\begin{align}
	(\nu_h - \nu_0) = \Delta \nu = a
\end{align}

\begin{align}
	L(\nu) = \dfrac{\Delta \nu^2}{ (\nu - \nu_0)^2 + \Delta \nu^2}
\end{align}

\begin{align}
	L(\lambda) = \dfrac{b^2}{ c^2(1/\lambda - 1/\lambda_0)^2 + b^2}
\end{align}

\begin{align}
	L(\lambda) = \dfrac{b^2}{ c^2 \left(\dfrac{\lambda - \lambda_0}{\lambda  \lambda_0}\right)^2 + b^2}
\end{align}

\begin{align}
	L(\lambda) = \dfrac{b^2 \lambda^2 \lambda_0^2}{c^2}
				\dfrac{1}{\left(\lambda - \lambda_0\right)^2 + \lambda^2 \lambda_0^2 b^2/c^2}
\end{align}

\begin{align}
	L(\lambda_0) = 1
\end{align}

\begin{align}
	L(\lambda_h) = \dfrac{1}{2} = \dfrac{b^2 \lambda_h^2 \lambda_0^2}{c^2}
\dfrac{1}{\left(\lambda_h - \lambda_0\right)^2 + \lambda_h^2 \lambda_0^2 b^2/c^2}
\end{align}

\begin{align}
	 2 \dfrac{b^2 \lambda_h^2 \lambda_0^2}{c^2}
				= \left(\lambda_h - \lambda_0\right)^2 + \lambda_h^2 \lambda_0^2 b^2/c^2
\end{align}

\begin{align}
	\dfrac{b^2 \lambda_h^2 \lambda_0^2}{c^2}
		= \left(\lambda_h - \lambda_0\right)^2
\end{align}

\begin{align}
	\dfrac{b^2}{c^2} = \left(\lambda_h - \lambda_0\right)^2 \dfrac{1}{\lambda_h^2 \lambda_0^2}
\end{align}

\begin{align}
	L = \left(\lambda_h - \lambda_0\right)^2 \dfrac{1}{\left(\lambda - \lambda_0\right)^2 + \left(\lambda_h - \lambda_0\right)^2}
\end{align}

\begin{align}
	\Delta \lambda_{hwhm} = \lambda - \lambda_0
\end{align}

\begin{align}
	L =   \dfrac{ \Delta \lambda^2}{\left(\lambda - \lambda_0\right)^2 + \Delta \lambda^2}
\end{align}

\begin{align}
   \int_{-\infty}^{-\infty} \dfrac{1}{1 + x^2} dx = \arctan(\infty) - \arctan(-\infty) = \pi
\end{align}


\begin{align}
	x &= \dfrac{\left(\lambda - \lambda_0\right)}{ \Delta \lambda} \\
	dx &= \dfrac{1}{\Delta \lambda} d\lambda
\end{align}

\begin{align}
	L =   \dfrac{\dfrac{1}{\pi} \Delta \lambda}{\left(\lambda - \lambda_0\right)^2 + \Delta \lambda^2}
\end{align}

\begin{align}
	L =  \dfrac{1}{\pi} \dfrac{\Delta \lambda}{\left(\lambda - \lambda_0\right)^2 + \Delta \lambda^2}
\end{align}

\begin{align}
	\int \dfrac{1}{\pi} \dfrac{\Delta \lambda}{\left(\lambda - \lambda_0\right)^2 + \Delta \lambda^2} d\lambda = 1
\end{align}

\begin{align}
	\int \dfrac{1}{\pi} \dfrac{\Delta \lambda}{\left(\lambda - \lambda_0\right)^2 + \Delta \lambda^2} d\lambda = 1
\end{align}


